progs/malloc_lemmas.v
@@ -31,7 +31,6 @@ Lemma int_add_repr_0_r: forall i, Int.add i (Int.repr 0) = i.
 Proof. intros. apply Int.add_zero. Qed.
 Hint Rewrite int_add_repr_0_l int_add_repr_0_r : normalize.
 
-
 Lemma field_storable_offset_zero:
   forall sh ty id v, 
    field_storable sh ty id (offset_val v (Int.repr 0)) =
@@ -48,36 +47,213 @@ Definition spacer (pos: Z) (alignment: Z) (v: val) : mpred :=
    memory_block Share.top (Int.repr (align pos alignment - pos))
                               (offset_val v (Int.repr pos)).
 
+Definition withspacer (pos: Z) (alignment: Z) (v: val) (P: mpred) : mpred :=
+   match align pos alignment - pos with
+   | Z0 => P
+   | n => memory_block Share.top (Int.repr n) (offset_val v (Int.repr pos)) * P
+   end.
+
+Lemma withspacer_spacer: forall pos alignment v P,
+   withspacer pos alignment v P = spacer pos alignment v * P.
+Proof.
+  intros.
+ unfold withspacer, spacer.
+ destruct (align pos alignment - pos); auto.
+ rewrite memory_block_zero, emp_sepcon; auto.
+Qed.
+
 Fixpoint malloc_assertion (pos: Z) (ty: type)  (v: val) : mpred :=
   match ty with
-  | Tstruct id fld a => spacer pos (alignof ty) v *
-                          malloc_assertion_fields 0 ty fld 
-                                    (offset_val v (Int.repr (align pos (alignof ty)))) 
-  | _ => spacer pos (alignof ty) v *
-                         memory_block Share.top (Int.repr (sizeof ty) )
-                            (offset_val v (Int.repr (align pos (alignof ty))))
+  | Tstruct id fld a => withspacer pos (alignof ty) v
+                          (malloc_assertion_fields 0 ty fld 
+                                    (offset_val v (Int.repr (align pos (alignof ty)))))
+  | _ => withspacer pos (alignof ty) v
+                         (memory_block Share.top (Int.repr (sizeof ty) )
+                            (offset_val v (Int.repr (align pos (alignof ty)))))
   end
 
 with malloc_assertion_fields (pos:Z) (t0: type) (flds: fieldlist) (v: val) : mpred :=
  match flds with
  | Fnil => emp
- | Fcons id ty flds' => spacer pos (alignof ty) v * 
-                                   field_storable Share.top t0 id 
-                                        (offset_val v (Int.repr (align pos (alignof ty)))) * 
+ | Fcons id ty flds' => withspacer pos (alignof ty) v 
+                                     (field_storable Share.top t0 id 
+                                          (offset_val v (Int.repr (align pos (alignof ty))))) * 
                                    malloc_assertion_fields pos t0 flds' v
   end.
 
-Ltac simpl_malloc_assertion :=
-  match goal with |- context [malloc_assertion ?N ?T ?V] =>
-    let MA := fresh "MA" in
-    remember (malloc_assertion  N T V) as MA;
-    match goal with H: MA = _ |- _ =>
-       simpl in H; try fold T in H;
-     unfold Zmax, align, spacer in H; simpl in H;
-     normalize in H;
-     subst MA
-    end
+
+Fixpoint reptype (ty: type) : Type :=
+  match ty with
+  | Tvoid => unit
+  | Tint _ _ _ => int
+  | Tfloat _ _ => float
+  | Tpointer t1 a => val
+  | Tarray t1 sz a => list (reptype t1)
+  | Tfunction t1 t2 => unit
+  | Tstruct id fld a => reptype_list prod fld
+  | Tunion id fld a => reptype_list sum fld
+  | Tcomp_ptr id a => unit
+  end
+
+with reptype_list (f: Type -> Type -> Type) (fld: fieldlist) : Type :=
+  match fld with
+  | Fnil => unit
+  | Fcons id ty fld' => f (reptype ty) (reptype_list f fld')
   end.
+
+Fixpoint arrayof (t: Type) (f: forall (v1: val) (v2: t),  mpred)
+         (t1: type) (ofs: Z) (v1: val) (v2: list t) : mpred :=
+    match v2 with
+    | v::rest => f (offset_val v1 (Int.repr ofs)) v * arrayof t f t1 (ofs + sizeof t1) v1 rest
+    | nil => emp
+   end.
+
+Definition maybe_field_mapsto (t: type) (sh: Share.t) (t_str: type) (id: ident) (pos: Z) (v: val) :
+                     (reptype t -> mpred) -> reptype t -> mpred :=
+match t as t0 return ((reptype t0 -> mpred) -> reptype t0 -> mpred) with
+| Tint i s a =>
+    fun (_ : reptype (Tint i s a) -> mpred) (v2'0 : reptype (Tint i s a)) =>
+    field_mapsto sh t_str id (offset_val v (Int.repr pos)) (Vint v2'0)
+| Tfloat f a =>
+    fun (_ : reptype (Tfloat f a) -> mpred) (v2'0 : reptype (Tfloat f a)) =>
+    field_mapsto sh t_str id (offset_val v (Int.repr pos)) (Vfloat v2'0)
+| Tpointer t0 a =>
+    fun _ =>  field_mapsto sh t_str id (offset_val v (Int.repr pos))
+| Tcomp_ptr _ _ =>
+    fun _ _ => field_storable sh t_str id (offset_val v (Int.repr pos))
+| t' => fun (alt1 : reptype t' -> mpred)  => alt1 
+end.
+
+Fixpoint typed_mapsto (t1: type) (sh: Share.t) (pos: Z) (v: val) (v2: reptype t1) : mpred :=
+match t1 as t return (t1 = t -> mpred) with
+| Tvoid => emp
+| Tint i s a =>
+    fun H : t1 = Tint i s a =>
+    let H0 :=
+      eq_rect_r (fun t2 : type => reptype t2 -> mpred)
+        (fun v3 : reptype (Tint i s a) =>
+                withspacer pos (alignof (Tint i s a)) v
+                (mapsto sh (Tint i s a) (offset_val v (Int.repr (align pos (alignof t1)))) (Vint v3))) H in
+    H0 v2
+| Tfloat f a =>
+    fun H : t1 = Tfloat f a =>
+    let H0 :=
+      eq_rect_r (fun t2 : type => reptype t2 -> mpred)
+        (fun v3 : reptype (Tfloat f a) =>
+                withspacer pos (alignof (Tfloat f a)) v
+                (mapsto sh (Tfloat f a) (offset_val v (Int.repr (align pos (alignof t1)))) (Vfloat v3))) H in
+    H0 v2
+| Tpointer t a => 
+    fun H : t1 = Tpointer t a =>
+    let H0 :=
+      eq_rect_r (fun t2 : type => reptype t2 -> mpred)
+        (fun v3 : reptype (Tpointer t a) =>
+                withspacer pos (alignof (Tpointer t a)) v
+                (mapsto sh (Tpointer t a) (offset_val v (Int.repr (align pos (alignof t1)))) v3)) H in
+    H0 v2
+| Tarray t z a =>
+    fun H : t1 = Tarray t z a =>
+    let H0 :=
+      eq_rect_r (fun t2 : type => reptype t2 -> mpred)
+        (fun v3 : reptype (Tarray t z a) => 
+                 withspacer pos (alignof t) v
+                 (arrayof _ (typed_mapsto t sh (align pos (alignof t))) t 0 v v3))
+        H in
+    H0 v2
+| Tfunction t t0 => emp
+| Tstruct i f a =>
+    fun H : t1 = Tstruct i f a =>
+    let H0 :=
+      eq_rect_r (fun t2 : type => reptype t2 -> mpred)
+        (fun v3 : reptype (Tstruct i f a) =>
+                 withspacer pos (alignof (Tstruct i f a)) v
+                 (structfieldsof (Tstruct i f a) f sh (align pos (alignof t1)) v v3)) H in
+    H0 v2
+| Tunion i f a =>
+    fun H : t1 = Tunion i f a =>
+    let H0 :=
+      eq_rect_r (fun t2 : type => reptype t2 -> mpred)
+        (fun v3 : reptype (Tunion i f a) =>
+                 withspacer pos (alignof (Tunion i f a)) v
+         (unionfieldsof f sh (align pos (alignof t1)) v v3)) H in
+    H0 v2
+| Tcomp_ptr i a => 
+        fun _ =>
+          withspacer pos (alignof (Tcomp_ptr i a)) v
+          (memory_block sh (Int.repr (sizeof (Tcomp_ptr i a))) (offset_val v (Int.repr pos)))
+end eq_refl
+ with
+ structfieldsof (t_str: type) (flds: fieldlist) (sh: Share.t) (pos: Z) (v: val) (v2: reptype_list prod flds) : mpred :=
+match flds as f0 return (flds = f0 -> mpred) with
+| Fnil => fun _ : flds = Fnil => emp
+| Fcons i t f0 =>
+    fun H : flds = Fcons i t f0 =>
+    let H0 :=
+      eq_rect_r (fun flds0 : fieldlist => reptype_list prod flds0 -> mpred)
+        (fun v3 : reptype_list prod (Fcons i t f0) =>
+         let (v2', vr) := v3 in
+            withspacer pos (alignof t) v
+            (maybe_field_mapsto t sh t_str i (align pos (alignof t)) v (typed_mapsto t sh (align pos (alignof t)) v) v2') *
+            structfieldsof t_str f0 sh pos v vr) H in
+    H0 v2
+end eq_refl
+ with
+unionfieldsof (flds: fieldlist) (sh: Share.t)  (pos: Z) (v: val) (v2: reptype_list sum flds) : mpred :=
+match flds as f0 return (flds = f0 -> mpred) with
+| Fnil => fun _ : flds = Fnil => emp
+| Fcons i t f0 =>
+    fun H : flds = Fcons i t f0 =>
+    let H0 :=
+      eq_rect_r (fun flds0 : fieldlist => reptype_list sum flds0 -> mpred)
+        (fun v3 : reptype_list sum (Fcons i t f0) =>
+         match v3 with
+         | inl v2' => typed_mapsto t sh pos v v2'
+         | inr vr =>  unionfieldsof f0 sh pos v vr 
+         end) H
+    in H0 v2
+end eq_refl.
+
+Lemma field_mapsto_offset_zero:
+  forall sh ty id v, 
+   field_mapsto sh ty id (offset_val v (Int.repr 0)) =
+   field_mapsto sh ty id v.
+Proof.
+ unfold field_storable; intros. extensionality v2.
+ destruct v; try solve [simpl; auto].
+ simpl offset_val. rewrite int_add_repr_0_r. reflexivity.
+Qed.
+Hint Rewrite field_mapsto_offset_zero: normalize.
+
+Ltac simpl_malloc_assertion' T H MA :=
+       unfold malloc_assertion, typed_mapsto, eq_rect_r, withspacer, align, Zmax in H;
+       simpl in H; try fold T in H;
+       repeat rewrite emp_sepcon in H; repeat rewrite sepcon_emp in H;
+       repeat rewrite field_storable_offset_zero in H;
+       repeat rewrite field_mapsto_offset_zero in H;
+     subst MA.
+
+Ltac simpl_malloc_assertion :=
+    let MA := fresh "MA" in
+  match goal with 
+  | |- context [malloc_assertion ?N ?T ?V] =>
+         remember (malloc_assertion  N T V) as MA;
+         match goal with H: MA = _ |- _ => simpl_malloc_assertion' T H MA end
+  | |- context [typed_mapsto ?T ?SH ?N ?V ?V'] =>
+         remember (typed_mapsto T SH N V V') as MA;
+         match goal with H: MA = _ |- _ => simpl_malloc_assertion' T H MA end
+  end.
+
+(* TESTING...
+Require Import progs.queue.
+Parameter sh: Share.t.
+Parameter v: val.
+Goal forall v2: reptype t_struct_elem, typed_mapsto t_struct_elem sh 0 v v2 =  emp.
+intros.
+simpl in v2.
+destruct v2 as [i [j [[] []]]].
+simpl_malloc_assertion.
+
+*)
 
 Lemma malloc_assert: forall ty, 
    memory_block Share.top (Int.repr (sizeof ty)) =
